Xlone-Seed.dfy
@@ -15,102 +15,54 @@ decreases *
     requires myBoundsOK(into, into)  //hmm
   requires forall x <- context :: x.Ready() && x.AllOutgoingReferencesWithinThisHeap(context)
 {
-  var m0 : Klon := seed(a, into, context);
+  var  rm := sheepKlon(a, into, context, proposeBounds(into));
 
-  assert m0.StupidCalidFragilistic();
-
-  var m1 : Klon;
-
-  reveal COK();
-
-  assert COK(a, m0.oHeap);
-  assert klonCanKV(m0,a,a);
-
-
-  b := new Object.make(a.fieldModes, m0.clowner, m0.oHeap, "clone_of_" + a.nick, m0.clbound);
-
-    assert m0.StupidCalidFragilistic();
-    assert a.Ready();
-    assert m0.ownersInKlown(a);
-    assert m0.o.Ready();
-    assert m0.objectInKlown(m0.o);
-    assert m0.CalidCanKey(a);
-    assert a !in m0.m.Keys;
-    assert b !in m0.m.Values;
-    assert a in m0.oHeap;
-    assert b.Ready() ;
-    assert b.Valid() ;
-    assert b.Context(m0.hns({b}));
-    assert m0.m.Keys <= m0.oHeap;
-    assert klonVMapOK(m0.m);
-    assert klonCanKV(m0,a,b);
-    assert m0.CalidLineKV(a,b);
-
-  assert m0.CKV_preconditions(a,b);
-  assert m0.CalidLineKV(a,b);
-
-  assert m0.StupidCalidFragilistic();
-  assert m0.ownersInKlown(m0.o);
-
-  m1 := m0.CalidKV(a,b);
-  assert a == m0.o == m1.o;
-  assert m1.o in m1.m.Keys;
-  assert m1.objectInKlown(m1.o);
-  assert m1.SuperCalidFragilistic();
-  var rm := Xlone_All_Fields(a,b,m1);
   assert rm.SuperCalidFragilistic();
+
   subtext := rm.hns();
+  b := rm.o;
 }
+//
+// lemma {:isolate_assertions} STOOPID(x : Object, oHeap : set<Object>)
+//    requires COK(x,oHeap)
+//     ensures reveal COK(); COK(x,oHeap) && x.Ready() && x.Valid() && x.Context(oHeap)
+//   {
+//   assert COK(x,oHeap);
+//   reveal COK();
+//   assert x.Ready() && x.Valid() && x.Context(oHeap);
+//   }
+//
+// lemma {:isolate_assertions} STOOPID_TREE(k : Object, v : Object, m : Klon)
+//  //catually NOT so stupid , cos there's NOT neceesedarily inside relkationshp bettwen k & v
+//    requires k == v
+//     ensures inside(k,v)
+// {}
 
-lemma {:isolate_assertions} STOOPID(x : Object, oHeap : set<Object>)
-   requires COK(x,oHeap)
-    ensures reveal COK(x); COK(x,oHeap) && x.Ready() && x.Valid() && x.Context(oHeap)
-  {
-  assert COK(x,oHeap);
-  reveal COK();
-  assert x.Ready() && x.Valid() && x.Context(oHeap);
-  }
 
-lemma {:isolate_assertions} STOOPID_TOO(m : Klon)
-   requires m.StupidCalidFragilistic()
-   requires m.objectInKlown(m.o)
-    ensures m.SuperCalidFragilistic()
-{}
-
-function {:isolate_assertions} {:timeLimit 15}  seed(o : Object, clowner : Owner, oHeap : set<Object>) : (m : Klon)
+  method {:isolate_assertions} {:timeLimit  30} sheepKlon(o : Object, clowner : Owner, oHeap : set<Object>, clbound : Owner := froposeBounds(clowner)) returns  (m : Klon)
 //seed Klon for cloning object o,  owner of clone being clowner, within heap oHeap...
+   decreases *
+    requires AllReady(clowner)
+    requires AllReady(clbound)
+    requires myBoundsOK(clowner, clbound)
     requires COK(o, oHeap)
     requires CallOK(oHeap)
     requires forall x <- oHeap :: x.Ready() && x.AllOutgoingReferencesWithinThisHeap(oHeap)
 
-    requires oHeap >= flatten(clowner) >= flatten(clowner)   //GRR
+    requires oHeap >= flatten(clowner) >= flatten(clbound) >= o.AMFB
     requires flatten(clowner) >= flatten(clowner)
     requires forall o <- flatten(clowner) :: o.Ready()
-    requires myBoundsOK(clowner, clowner)
-    requires myBoundsOK(o.owner, o.bound)  //GRR update ready?
 
     ensures (m.m.Keys <= m.oHeap)
     ensures (m.m.Values <= m.hns())
-    ensures (m.ownersReadyInKlown(o))  //not obejctReadyInCloneapparentlyt...  FUCK need to look at Xlone-MAIN I BET
     ensures (m.HeapOwnersReady())
     ensures (m.c_amfx <= m.oHeap)
     ensures forall x <- oHeap :: (x.Ready() && x.Valid() && x.Context(oHeap))
 
-    ensures m.StupidCalidFragilistic() /// cos obkject aint in the KLON at this ponmt..
     ensures COK(o, m.oHeap)
-//    ensures allMapOwnersThruKlownIfInsideOK(m)
-//
-//     ensures m == Klon( (map x <- o.AMFX :: x),
-//         o,
-//         o.AMFX,
-//         clowner,
-//         flatten(clowner),
-//         (flatten(clowner) - mapThruKlon(o.AMFX, m)),
-//         (mapThruKlon(o.AMFX, m) - flatten(clowner)),
-//         oHeap,
-//         {} )
+    ensures m.SuperCalidFragilistic()
 
-    reads oHeap`fields, oHeap`fieldModes
+//    reads oHeap`fields, oHeap`fieldModes
     {
      assert CallOK(oHeap); reveal CallOK(); reveal COK();
      assert forall x <- oHeap :: (reveal COK(); COK(x,oHeap));
@@ -132,99 +84,251 @@ function {:isolate_assertions} {:timeLimit 15}  seed(o : Object, clowner : Owner
     forall x <- mep.Keys ensures true //by
       {
         assert x.Ready();
+        assert x.Valid();
         assert outside(x,o);
         assert (inside(x,o)) ==> (mep[x] !in oHeap);
         assert x in oHeap;
+        assert x == mep[x];
+        assert mep[x].Ready();
+        assert x.Context(oHeap);
+        assert x.Context(oHeap+mep.Values);
 
         //assert mep0.Keys >= o.AMFX >= o.AMFB;
         //assert mep0.Keys >= mep0[o].AMFX >= mep0[o].AMFB;
       }
-    var mTKoA := mapThruVMap(o.AMFX, mep);
-    var oxtra := mTKoA - clamfx;
-    var cxtra := clamfx - mTKoA;
+    // var mTKoA := mapThruVMap(o.AMFX, mep);
+    // var oxtra := mTKoA - clamfx;
+    // var cxtra := clamfx - mTKoA;
+
+
+  reveal COK();
+
+  assert COK(o, oHeap);
+
+
+ var c := new Object.make(o.fieldModes, clowner, oHeap, "clone_of_" + o.nick, clbound);
+
+assert c.Ready();
+assert c.Valid();
+assert c.Context(oHeap+{c});
+assert c.fieldModes == o.fieldModes;
+
+
+forall x <- oHeap ensures (x.Context(oHeap+{c}))
+ { reveal COK();
+   assert COK(x,oHeap);
+   assert x.Ready();
+   assert x.Valid();
+   assert x.Context(oHeap);
+   x.WiderContext(oHeap,oHeap+{c});
+   assert x.Context(oHeap+{c});
+ }
+
+
+   assert AllReady(mep.Keys);
+   assert AllReady(mep.Values);
+
+//put o := into the map
+   var me := map2vmap(mep[o:=c]);
+   assert AllMapEntriesAreUnique(me);
 
 
 
-    var m : Klon := Klon(mep,
+assert forall x <- me.Keys ::
+(if (x == o)  then ((me[x] == c) && (c.Ready()))
+              else ((me[x] == x) && (x.Ready()))
+) && me[x].Ready();
+
+
+assert forall x <- me.Keys ::
+(if (x == o)  then ((me[x] == c) && (c.Context(oHeap+{c})))
+              else ((me[x] == x) && (x.Context(oHeap+{c})))
+) && me[x].Context(oHeap+{c});
+
+assert forall x <- me.Keys ::
+(if (x == o)  then ((me[x] == c) && (c.fieldModes == o.fieldModes))
+              else ((me[x] == x) && (me[x].fieldModes == x.fieldModes))
+) && (me[x].fieldModes == x.fieldModes);
+
+assert inside(o,o);
+assert forall k <- me.Keys :: (not(inside(k,o)) ==> (me[k] == k));
+assert forall x <-  me.Values :: x.Context(me.Values+oHeap);
+
+
+//
+// assert forall k : Object <- me.Keys :: ( && (k.Ready()) && (objectInKlown(k)) && (me[k].Ready()) && (me[k] in hns()) );
+//
+// assert forall k <- me.Keys :: CalidLineKV(k, me[k]);
+//
+// assert forall x <- me.Values :: (x.AMFO <= hns());
+
+
+assert forall k <- me.Keys :: ( (inside(k,o)) ==> (me[k] !in oHeap));
+
+   assert AllReady(me.Keys);
+   assert AllReady(me.Values);
+
+    var m0 : Klon := Klon(me,
                             o,
-//                          o.AMFX,
+                            c,
                             clowner,
-                            proposeBounds(clowner),
-                            // clamfx,
-                            // oxtra,
-                            // cxtra,
+                            clbound,
                             oHeap,
                             o.AMFX,
+                            flatten(clbound),
                             clamfx);
+assert inside(o, o);
+assert inside(c, c);
+assert inside(m0.o, m0.o);
+assert inside(m0.m[m0.o], m0.m[m0.o]);
+assert outside(m0.o, m0.o) <==> (m0.o == m0.m[m0.o]);
+assert inside(m0.o, m0.o) <==> inside(m0.m[m0.o], m0.m[m0.o]);
+assert inside(m0.m[m0.o], m0.m[m0.o]);
 
-// assert forall x <- m.m.Keys :: (
-//     && (outside(x,m.o))
-//     && (x.AMFX <= m.m.Keys)
-//     && (x.AMFB <= m.m.Keys)
-// //    && (k.bound <= k.owner <= m.Keys)
-//     && (m.ownersInKlown(x))  //belt and braces--- currently a requirement!
-//
-//   && (x.Ready())
-//   && (m.ownersInKlown(x))
-//   && (x.Ready())
-//   && (m.apoCalidse())
-//   && (x.owner <= m.m.Keys <= m.oHeap)
-//   && (m.m.Values <= flatten( m.hns() ))
-//   && (m.o.Ready())
-//   && (m.HeapOwnersReady())
-//   && (m.c_amfx <= m.oHeap)
-//
-//     && (checkOwnershipOfClone(x,x,m))
-//     && (checkBoundOfClone(x,x,m))
-//     && (mappingOwnersThruKlownKV(x,x,m))
-// );
+assert HighLineKV(o, c, m0);
 
+assert m0.m.Values == me.Values;
+assert forall x <-  me.Values :: x.Context(me.Values+oHeap);
+assert forall x <-  m0.m.Values :: x.Context(m0.hns());
 
-forall x <- m.m.Keys ensures (true) //GRRR (m.CalidLineKV(x,x)) //by
-{
-    assert (outside(x,m.o));
-    assert (x.AMFX <= m.m.Keys);
-    assert (x.AMFB <= m.m.Keys);
-    assert (m.ownersInKlown(x)) ;
-    assert (x.Ready());
-    assert (m.ownersInKlown(x));
-    assert (x.Ready());
-//    assert (m.apoCalidse());
-    assert (x.owner <= m.m.Keys <= m.oHeap);
-    assert (m.m.Values <= flatten( m.hns() ));
-    assert (m.o.Ready());
-    assert (m.HeapOwnersReady());
-    assert (m.c_amfx <= m.oHeap);
-    assert (checkOwnershipOfClone(x,x,m));
-    assert (checkBoundOfClone(x,x,m));
-    assert (mappingOwnersThruKlownKV(x,x,m));
+forall k <- m0.m.Keys ensures (m0.gettingThere()) {
+   if (k == c) {
+      assert (k.Ready()) && (m0.objectInKlown(k)) && (m0.m[k].Ready()) && (m0.m[k] in m0.hns());
+   } else {
+      assert (k.Ready()) && (m0.objectInKlown(k)) && (m0.m[k].Ready()) && (m0.m[k] in m0.hns());
+
+   }
 }
 
-// assert forall x <- m.m.Keys :: m.CalidLineKV(x,x);
 
 
-  // assert m.hns() == oHeap + clamfx;
-    assert m.oHeap == oHeap;
+forall k <- m0.m.Keys ensures (m0.CalidLineKV(k, m0.m[k])) {
+  if (k == c) {
 
-    assert o.AMFX == m.o_amfx <= m.m.Keys;
+  } else {
 
-    assert COK(o, oHeap);   reveal COK();
-    assert COK(o, m.oHeap);
-
-    assert m.oHeap == oHeap;
-
-    assert CallOK(oHeap);
-    assert forall x <- oHeap :: x.Ready();
-
-    assert m.o.Ready();
-    assert (m.o.AMFX <= m.m.Keys);
+  }
+}
 
 
-    assert (m.m.Keys <= m.oHeap);
-    assert (m.m.Values <= m.hns());
-    assert (m.ownersReadyInKlown(o));
-    assert (m.HeapOwnersReady());
-    assert (m.c_amfx <= m.oHeap);
+assert m0.AllLinesCalid();
+assert m0.gettingThere();
+assert m0.SuperCalidFragilistic();
+//m := m0;
+m := Xlone_All_Fields(o,c,m0);
+}
 
-    m
-    }
+// //  forall x <- m.m.Keys ensures (true)  {
+// // //    assert (outside(x,m.o)); //where the FUCK did this come from?
+// //     assert (x.AMFX <= m.m.Keys);
+// //     assert (x.AMFB <= m.m.Keys);
+// //     assert (m.ownersInKlown(x));
+// //     assert (x.Ready());
+// //     assert (m.apoCalidse());
+// //
+// //   assert (x.owner <= m.m.Keys <= m.oHeap);
+// //   assert (m.m.Values <= flatten( m.hns() ));
+// //   assert (m.o.Ready());
+// //   assert (m.HeapOwnersReady());
+// //   assert (m.c_amfx <= m.oHeap);
+// //   assert m.m[x].Ready();
+// //     assert (checkOwnershipOfClone(x,m.m[x],m));
+// //     assert (checkBoundOfClone(x,m.m[x],m));
+// //     assert (mappingOwnersThruKlownKV(x,m.m[x],m));
+// //  }
+//
+//
+// forall k <- m0.m.Keys ensures (true) {
+//      assert (k.Ready());
+//      assert (m0.objectInKlown(k));
+//      assert (m0.m[k].Ready());
+//      assert (m0.m[k] in m0.hns());
+// }
+//
+// forall k <- m0.m.Keys ensures (HighLineKV(k, m0.m[k], m0)) {
+//   if (k == o) {
+//     assert m0.m[k] == c;
+//     assert HighLineKV(o, c, m0);
+//   } else {
+//     assert m0.m[k] == k;
+//     assert HighLineKV(k, m0.m[k], m0);
+//   }
+// }
+//
+//   assert m0.AllLinesCalid();
+//   assert m0.gettingThere();
+//   assert m0.SuperCalidFragilistic();
+//
+//  m := Xlone_All_Fields(o,c,m0);
+//
+//
+// // assert forall x <- m.m.Keys :: (
+// //     && (outside(x,m.o))
+// //     && (x.AMFX <= m.m.Keys)
+// //     && (x.AMFB <= m.m.Keys)
+// // //    && (k.bound <= k.owner <= m.Keys)
+// //     && (m.ownersInKlown(x))  //belt and braces--- currently a requirement!
+// //
+// //   && (x.Ready())
+// //   && (m.ownersInKlown(x))
+// //   && (x.Ready())
+// //   && (m.apoCalidse())
+// //   && (x.owner <= m.m.Keys <= m.oHeap)
+// //   && (m.m.Values <= flatten( m.hns() ))
+// //   && (m.o.Ready())
+// //   && (m.HeapOwnersReady())
+// //   && (m.c_amfx <= m.oHeap)
+// //
+// //     && (checkOwnershipOfClone(x,x,m))
+// //     && (checkBoundOfClone(x,x,m))
+// //     && (mappingOwnersThruKlownKV(x,x,m))
+// // );
+//
+//
+// assert m.SuperCalidFragilistic();
+//
+// forall x <- m.m.Keys ensures (m.CalidLineKV(x,m.m[x])) //GRRR (m.CalidLineKV(x,m.m[x])) //by
+// {
+//    // assert (outside(x,m.o));
+//     assert (x.AMFX <= m.m.Keys);  //???
+//     assert (x.AMFB <= m.m.Keys); //???
+//       assert (m.ownersInKlown(x)) ; //???
+//     assert (x.Ready()); //??? //??? //??? //??? //??? //???
+//     assert (m.ownersInKlown(x));
+//     assert (x.Ready());
+// //    assert (m.apoCalidse());
+//     assert (x.owner <= m.m.Keys <= m.oHeap);  //???
+//     assert (m.m.Values <= flatten( m.hns() ));
+//     assert (m.o.Ready()); //???
+//     assert (m.HeapOwnersReady()); //???
+//     assert (m.c_amfx <= m.oHeap);            //???
+//     assert (checkOwnershipOfClone(x,m.m[x],m));        //???        //???
+//     assert (checkBoundOfClone(x,m.m[x],m));
+//     assert (mappingOwnersThruKlownKV(x,m.m[x],m)); //???
+// }
+//
+// // // assert forall x <- m.m.Keys :: m.CalidLineKV(x,x);
+// //
+// //
+// //   // assert m.hns() == oHeap + clamfx;
+// //     assert m.oHeap == oHeap;
+// //
+// //     assert o.AMFX == m.o_amfx <= m.m.Keys;
+// //
+// //     assert COK(o, oHeap);   reveal COK();
+// //     assert COK(o, m.oHeap);
+// //
+// //     assert m.oHeap == oHeap;
+// //
+// //     assert CallOK(oHeap);
+// //     assert forall x <- oHeap :: x.Ready();
+// //
+// //     assert m.o.Ready();
+// //     assert (m.o.AMFX <= m.m.Keys);
+// //
+// //
+// //     assert (m.m.Keys <= m.oHeap);
+// //     assert (m.m.Values <= m.hns());
+// //     assert (m.ownersReadyInKlown(o));
+// //     assert (m.HeapOwnersReady());
+// //     assert (m.c_amfx <= m.oHeap);
